partial tree list lemmas

TreeLemmas.v
@@ -8,7 +8,6 @@ Require Export MST.SetLogic.
 Open Scope uset_scope.
 
 
-
 (* Graph vertex list *)
 
 Lemma V_in_graph_list :
@@ -98,14 +97,143 @@ Qed.
 
 
 
-(* Graph edge list *)
+(* Graph arc/edge list *)
+
+Lemma A_in_graph_list :
+	forall {V A} a (G: Graph V A), a ∈ A -> In a (GA_list V A G).
+Proof.
+	intros V A a G. generalize dependent a. induction G.
+	- intros a Ha. inversion Ha.
+	- intros arc Harc. simpl. apply IHG. assumption.
+	- intros arc Harc. simpl. inversion Harc.
+		+ subst. inversion H.
+			* left. reflexivity.
+			* right. left. reflexivity.
+		+ right. right. apply IHG. assumption.
+	- intros arc Harc. simpl. apply IHG. subst. assumption.
+Qed.
 
 Lemma E_in_graph_list :
-	forall {V E} {x y} (G: Graph V E), (x -- y) ∈ E -> In (x -- y) (GA_list V E G).
+	forall {V E} x y (G: Graph V E), (x -- y) ∈ E -> E_in (x ~~ y) (GE_list V E G).
 Proof.
-	intros V E x y G. generalize dependent y. generalize dependent x. induction G.
-	- intros x y Hxy. inversion Hxy.
-	- 
+	intros V E x y G. generalize dependent y. generalize dependent x.
+	induction G; intros p q H_pq; simpl in H_pq.
+	- inversion H_pq.
+	- apply IHG. assumption.
+	- simpl. case (E_eq_dec (p ~~ q) (x ~~ y)); intros H.
+		+ constructor.
+		+ apply IHG. inversion H_pq; subst.
+			* inversion H0; subst; exfalso; apply H; constructor.
+			* assumption.
+	- simpl. apply IHG. subst. assumption.
+Qed.
+
+Lemma A_in_list_graph :
+	forall {V A} a (G: Graph V A), In a (GA_list V A G) -> a ∈ A.
+Proof.
+	intros V A a G. generalize dependent a.
+	induction G; intros arc Harc; simpl in Harc.
+	- inversion Harc.
+	- apply IHG. assumption.
+	- destruct Harc as [Harc | Harc].
+		+ constructor. inversion Harc. subst. constructor.
+		+ destruct Harc as [Harc | Harc].
+			* inversion Harc; subst. constructor. constructor 2.
+			* constructor 2. apply IHG. assumption.
+	- subst. apply IHG. assumption.
+Qed.
+
+Lemma E_in_list_graph :
+	forall {V E} x y (G: Graph V E), E_in (x ~~ y) (GE_list V E G) -> (x -- y) ∈ E \/ (y -- x) ∈ E.
+Proof.
+	intros V E x y G. generalize dependent y. generalize dependent x.
+	induction G; intros p q H_pq; simpl in H_pq.
+	- inversion H_pq.
+	- apply IHG. assumption.
+	- generalize dependent H_pq. case (E_eq_dec (p ~~ q) (x ~~ y)); intros H_pq H.
+		+ inversion H_pq; subst; [left | right]; repeat constructor.
+		+ apply IHG in H. inversion H; [left | right]; constructor 2; assumption.
+	- subst. apply IHG. assumption.
+Qed.
+
+Lemma E_in_symmetry :
+	forall x y E_lst, E_in (x ~~ y) E_lst -> E_in (y ~~ x) E_lst.
+Proof.
+	intros x y E_lst. generalize dependent y. generalize dependent x.
+	induction E_lst; intros.
+	- contradiction.
+	- simpl in H. generalize dependent H. case (E_eq_dec (x ~~ y) a); intros Hxy H.
+		+ inversion Hxy; subst; simpl.
+			* case (E_eq_dec (y ~~ x) (x ~~ y)); intros Hyx.
+				-- constructor.
+				-- exfalso. apply Hyx. apply E_rev.
+			* case (E_eq_dec (y ~~ x) (y ~~ x)); intros Hyx.
+				-- constructor.
+				-- exfalso. apply Hyx. constructor.
+		+ simpl. case (E_eq_dec (y ~~ x) a); intros Hyx.
+			* inversion Hyx; subst; constructor.
+			* apply IHE_lst. assumption.
+Qed.
+
+Lemma A_in_graph_iff_list :
+	forall {V A} x y (G: Graph V A), (x -- y) ∈ A <-> In (x -- y) (GA_list V A G).
+Proof. intros. split; [apply A_in_graph_list | apply A_in_list_graph]. Qed.
+
+Lemma E_in_graph_iff_list :
+	forall {V E} x y (G: Graph V E), E_in (x ~~ y) (GE_list V E G) <-> (x -- y) ∈ E \/ (y -- x) ∈ E.
+Proof.
+	intros. split; intros H.
+	- apply E_in_list_graph in H. assumption.
+	- destruct H.
+		+ apply E_in_graph_list. assumption.
+		+ apply E_in_symmetry. apply E_in_graph_list. assumption.
+Qed.
+
+
+(* 
+(* Tree arc list *)
+
+Fixpoint TA_list {V : V_set} {E : A_set} (T : Tree V E) {struct T} : A_list :=
+	match T with
+		| T_root r => A_nil
+		| T_leaf v e t f n _ _ => (n -- f) :: TA_list t
+		| T_eq v v' a a' _ _ t => TA_list t
+	end.
+
+Lemma A_in_tree_list :
+	forall {V A} x y (T: Tree V A), (x -- y) ∈ A -> In (x -- y) (TA_list T).
+Proof.
+	intros V A x y T. generalize dependent y. generalize dependent x.
+	induction T; intros p q H_pq; simpl in H_pq.
+	- inversion H_pq.
+	- simpl. destruct H_pq as [arc | arc].
+		+ left. 
+	- inversion Hx.
+		+ inversion H. subst. constructor. reflexivity.
+		+ subst. constructor 2. apply IHT. assumption.
+	- apply IHT. subst. assumption.
+Qed.
+
+Lemma V_in_list_tree :
+	forall {V E} x (T: Tree V E), In x (TV_list T) -> x ∈ V.
+Proof.
+	intros V E x T. generalize dependent x. induction T; intros x Hx.
+	- inversion Hx.
+		+ subst. constructor.
+		+ inversion H.
+	- inversion Hx.
+		+ subst. constructor. constructor.
+		+ constructor 2. apply IHT. assumption.
+	- simpl TV_list in Hx. subst. apply IHT. assumption.
+Qed.
+
+Lemma V_in_tree_iff_list :
+	forall {V E} x (T: Tree V E), x ∈ V <-> In x (TV_list T).
+Proof. intros. split; [apply V_in_tree_list | apply V_in_list_tree]. Qed.
+
+
+
+
 
 
 
@@ -114,7 +242,7 @@ Proof.
 
 Theorem tree_paths :
 	forall {V: V_set} {E: A_set} (T: Tree V E) x y,
-	x ∈ V -> y ∈ V -> exists (vl : V_list) (el : E_list), Path V E x y vl el.
+	x ∈ V -> y ∈ V -> exists (vl : V_list) (el : E_list), Path V E x y vl el. *)
 
 
 
